Kernel API work

Covalence/KernelAPI.lean
@@ -1,5 +1,17 @@
 import Covalence.Rewrite
 
+theorem Ctx.IsTy.rw_congr {Γ : Ctx} {A B : Tm} (h : Γ.IsTy A) (hab : Γ.Rw A B) : Γ.IsTy B
+  := have ⟨ℓ, h⟩ := h; sorry
+
+def Ctx.IsUniv (Γ : Ctx) (a : Tm) : Prop
+  := ∃ℓ, Γ.Rw a (.univ ℓ)
+
+theorem Ctx.IsUniv.rw_congr {Γ : Ctx} {a b : Tm} (h : Γ.IsUniv a) (hab : Γ.Rw a b) : Γ.IsUniv b
+  := have ⟨ℓ, h⟩ := h; ⟨ℓ, hab.symm.trans h⟩
+
+def Ctx.RwCmp (Γ : Ctx) (a b : Tm) : Prop
+  := Γ.Rw a b ∨ ∃A, Γ.Cmp A a b
+
 def Ctx.HasTyUnder (Γ : Ctx) (A B b : Tm) : Prop
   := ∃L : Finset ℕ, ∀x ∉ L, (Γ.cons x A).HasTy (B.bs0 (.fv x)) (b.bs0 (.fv x))
 
@@ -16,14 +28,20 @@ theorem Ctx.HasTyUnder.has_ty {Γ : Ctx} {A B b : Tm}
   have ⟨_, h⟩ := h;
   hA.pi_cf (ℓ := 0) (fun x hx => (h x hx).has_ty) rfl
 
--- theorem Ctx.HasTyUnder.of_has_ty {Γ : Ctx} {A B b : Tm}
---   (h : Γ.HasTy (.univ 0) (.pi 0 A (.has_ty b B))) : Γ.HasTyUnder A B b := by
---   have ⟨W, hAB, hW⟩ := h.outer_ty;
---   cases hAB with
---   | pi_cf hA hB hℓ =>
---   simp [Nat.imax] at hℓ
---   rename Finset ℕ => L
---   exists L
---   intro x hx
---   apply HasTy.of_has_ty
---   sorry
+theorem Ctx.HasTyUnder.of_has_ty {Γ : Ctx} {A B b : Tm}
+  (h : Γ.HasTy (.univ 0) (.pi 0 A (.has_ty b B))) : Γ.HasTyUnder A B b := by
+  have ⟨W, hAB, hW⟩ := h.outer_ty;
+  cases hAB with
+  | pi_cf hA hB hℓ =>
+  simp [Nat.imax] at hℓ
+  rename Finset ℕ => L
+  exists L
+  intro x hx
+  apply HasTy.of_has_ty
+  have ⟨W, hB', hW⟩ := (hB x hx).outer_ty
+  cases hB' with
+  | has_ty' hB' hb' => exact HasTy.has_ty_regular hb'
+
+theorem Ctx.HasTyUnder.has_ty_iff {Γ : Ctx} {A B b : Tm}
+  : Γ.HasTyUnder A B b ↔ Γ.HasTy (.univ 0) (.pi 0 A (.has_ty b B)) :=
+  ⟨Ctx.HasTyUnder.has_ty, Ctx.HasTyUnder.of_has_ty⟩
